Implement primitive extraction of constant expressions

Extraction/Core.lean
@@ -3,13 +3,29 @@ open Lean Meta Elab Term Tactic Grind
 
 namespace Lean.Meta.Grind.Extraction
 
-def extractMinAST (target : Expr) : GoalM (Expr × Expr) := do
-  let target ← shareCommon target
+-- Note: Expects `target` to be internalized.
+def extractMinAST (target : Expr) : GoalM Expr := do
   let min ← foldEqc target target fun node min => do
     let expr := node.self
     if expr.isFalse then return min
     if expr.sizeWithoutSharing < min.sizeWithoutSharing then return expr else return min
-  return (target, min)
+  return min
+
+-- Note: Expects `target` and `e` to be internalized.
+def extractExpr? (target e : Expr) : GoalM (Option Expr) := do
+  -- TODO: Support mvars.
+  unless ← isEqv target e do return none
+  return e
+
+def extractMain? (target : Expr) : Sketch → GoalM (Option Expr)
+  | .minAST => do
+    let min ← extractMinAST target
+    return min
+  | .expr e => do
+    let e ← shareCommon e
+    extractExpr? target e
+  | _ =>
+    throwError "`grind extract` currently only supports the `min_ast` and expression sketches"
 
 structure Extracted where
   /-- The result of extraction: the extracted term, equivalent to the proof goal. -/
@@ -17,8 +33,9 @@ structure Extracted where
   /-- Proves `result = target`/`result ≍ target`. -/
   eqHEqProof : Expr
 
-def extract (target : Expr) (sketch : Sketch) : GoalM (Option Extracted) := do
-  let .minAST := sketch | throwError "`grind extract` currently only supports the `min_ast` sketch"
-  let (internalizedTarget, result) ← extractMinAST target
-  let eqHEqProof ← mkEqHEqProof result internalizedTarget
+-- Note: This is expected to be run in the context of the failed grind goal, and with `target`
+--       being internalized.
+def extract? (target : Expr) (sketch : Sketch) : GoalM (Option Extracted) := do
+  let some result ← extractMain? target sketch | return none
+  let eqHEqProof ← mkEqHEqProof result target
   return some { result, eqHEqProof }
